#for training exercises at https://docs.kurrawong.ai. this vocab is intentionally missing various elements that are added through exercises.

@prefix : <http://example.com/pestRiskPath/> .
@prefix skos: <http://www.w3.org/2004/02/skos/core#> .

:0cade264-c648-4417-be04-063e9ca458b1 a skos:Concept ;
    skos:definition "Dispersal of pests by animals."@en ;
    skos:inScheme <http://example.com/pestRiskPath> ;
    skos:prefLabel "Animal dispersal"@en ;
    skos:topConceptOf <http://example.com/pestRiskPath> .

:157a5f8d-49ba-4666-9ae6-1be40d7ac6c7 a skos:Concept ;
    skos:prefLabel "Spore dispersal"@en .

:3a0b843e-665b-4c2e-b8a6-e97a572cf58e a skos:Concept ;
    skos:broader :2687143e-8f91-4c7a-8caa-e387cfea7ad8 ;
    skos:definition "Cargo"@en ;
    skos:inScheme <http://example.com/pestRiskPath> ;
    skos:prefLabel "Cargo"@en .

:81df7d51-87ba-43e7-9f5c-b192dd5b4b64 a skos:Concept ;
    skos:definition "Plants that support the growth and development of pests, acting as a source of food, shelter, and sometimes even a breeding ground."@en ;
    skos:inScheme <http://example.com/pestRiskPath> ;
    skos:prefLabel "Plant hosts"@en .

:2687143e-8f91-4c7a-8caa-e387cfea7ad8 a skos:Concept ;
    skos:definition "Dispersal of pests through various activities, including the intentional and unintentional transport of commodities, plants, and other items."@en ;
    skos:prefLabel "Human dispersal"@en .

:c380542f-21b3-475e-8fd0-cbcb48aff26e a skos:Concept ;
    skos:definition "Wildlife trafficking refers to the exchange of products derived from non-domesticated animals or plants usually extracted from their natural environment or raised under controlled conditions. "@en ;
    skos:prefLabel "Wildlife trafficking" ;
    skos:inScheme <http://example.com/pestRiskPath> ;
    skos:topConceptOf <http://example.com/pestRiskPath> .

<http://example.com/pestRiskPath> a skos:ConceptScheme ;
    skos:prefLabel "Pest Risk Pathway"@en .
